\documentclass[a4paper,12pt]{article}
\setlength{\parindent}{0cm}
\usepackage{amsmath, amssymb, amsthm, mathtools,pgfplots,bbm}
\usepackage{graphicx,caption}
\usepackage{verbatim}
\usepackage{venndiagram}
\usepackage[cm]{fullpage}
\usepackage{fancyhdr}
\usepackage{tikz}
\usepackage{listings}
\usepackage{color,enumerate,framed}
\usepackage{color,hyperref}
\definecolor{darkblue}{rgb}{0.0,0.0,0.5}
\hypersetup{colorlinks,breaklinks,
            linkcolor=darkblue,urlcolor=darkblue,
            anchorcolor=darkblue,citecolor=darkblue}

%\usepackage{tgadventor}
%\usepackage[nohug]{diagrams}
\usepackage[T1]{fontenc}
%\usepackage{helvet}
%\renewcommand{\familydefault}{\sfdefault}
%\usepackage{parskip}
%\usepackage{picins} %for \parpic.
%\newtheorem*{notation}{Notation}
%\newtheorem{example}{Example}[section]
%\newtheorem*{problem}{Problem}
\theoremstyle{definition}
%\newtheorem{theorem}{Theorem}
%\newtheorem*{solution}{Solution}
%\newtheorem*{definition}{Definition}
%\newtheorem{lemma}[theorem]{Lemma}
%\newtheorem{corollary}[theorem]{Corollary}
%\newtheorem{proposition}[theorem]{Proposition}
%\newtheorem*{remark}{Remark}
%\setcounter{section}{1}

\newtheorem{thm}{Theorem}[section]
\newtheorem{lemma}[thm]{Lemma}
\newtheorem{prop}[thm]{Proposition}
\newtheorem{cor}[thm]{Corollary}
\newtheorem{defn}[thm]{Definition}
\newtheorem*{examp}{Example}
\newtheorem{conj}[thm]{Conjecture}
\newtheorem{rmk}[thm]{Remark}
\newtheorem*{nte}{Note}
\newtheorem*{notat}{Notation}

%\diagramstyle[labelstyle=\scriptstyle]

\lstset{frame=tb,
  language=Oz,
  aboveskip=3mm,
  belowskip=3mm,
  showstringspaces=false,
  columns=flexible,
  basicstyle={\small\ttfamily},
  breaklines=true,
  breakatwhitespace=true,
  tabsize=3
}


\pagestyle{fancy}




\fancyhead{}
\renewcommand{\headrulewidth}{0pt}

\lfoot{\color{black!60}{\sffamily Zhangsheng Lai}}
\cfoot{\color{black!60}{\sffamily Last modified: \today}}
\rfoot{\textsc{\thepage}}



\begin{document}
\flushright{Zhangsheng Lai\\1002554}
\section*{Real Analysis: Homework 5}

\begin{enumerate}
\item 
\begin{enumerate}[(a)]
\item
\begin{align*}
\frac{\partial}{\partial \epsilon}F(\epsilon,t) &= \int_{0}^{\infty}\frac{\partial}{\partial \epsilon}e^{-\epsilon x}\frac{\sin xt}{x}\,dx\\\
&=-\int_{0}^{\infty}e^{-\epsilon x} \sin xt\, dx\\
&=-\left\{\left[\sin xt\cdot -\frac{1}{\epsilon}e^{-\epsilon x}\right]_{0}^{\infty}-\int_{0}^{\infty}-\frac{1}{\epsilon}e^{-\epsilon x} t \cos xt \, dx\right\}\\
&=-\frac{t}{\epsilon}\int_{0}^{\infty}e^{-\epsilon x} \cos xt \, dx\\
&=-\frac{t}{\epsilon}\left\{\left[\cos xt \cdot -\frac{1}{\epsilon}e^{-\epsilon x}\right]_{0}^{\infty}-\int_{0}^{\infty}-\frac{1}{\epsilon}e^{-\epsilon x}\cdot -t \sin xt \, dx\right\}\\
&=\frac{t}{\epsilon^2}+\frac{t^2}{\epsilon^2}\int_{0}^{\infty}e^{-\epsilon x} \sin xt \, dx\\
\end{align*}
with some algebraic manipulation we obtain
\begin{align*}
\int_{0}^{\infty}e^{-\epsilon x} \sin xt \, dx = -\frac{t}{t^2+\epsilon^2}
\end{align*}

\item
We observe that
\begin{align*}
\left|e^{-\epsilon x}\frac{\sin xt}{x}\right| \leq \frac{e^{-\epsilon x}}{x}
\end{align*}
thus
\begin{align*}
\sup_{x,t \in \mathbb{R}}\left|e^{-\epsilon x}\frac{\sin xt}{x} - 0\right| \to 0 \text{ as } \epsilon \to \infty 
\end{align*}
Hence,
\begin{align*}
\lim_{\epsilon \to \infty}F(\epsilon,t) = \int_{0}^{\infty}\lim_{\epsilon \to \infty}e^{-\epsilon x}\frac{\sin xt}{x}\,dx=0
\end{align*}



\item 
As $e^{-\epsilon x}\frac{\sin xt}{x}$ is nonnegative, converges uniformly to $\frac{\sin xt}{x}$ as $\epsilon \to 0$, by Monotone convergence theorem, we have 
\begin{align}
\lim_{\epsilon \to 0}F(\epsilon,t) &= \int_{0}^{\infty}\frac{\sin xt}{x}\,dx \nonumber \\
&= \int_{0}^{\infty}\int_{0}^{\infty}e^{-xy}\sin xt\,dy\,dx \nonumber \\
&= \int_{0}^{\infty}\left(\int_{0}^{\infty}e^{-xy}\sin xt\,dx\right)\,dy \label{eq1}
\end{align}
we work on the inner integral first,
\begin{align*}
\int_{0}^{\infty}e^{-xy}\sin xt\,dx&=\left[\sin xt -\frac{1}{y}e^{-xy}\right]_{0}^{\infty}-\int_{0}^{\infty}-\frac{1}{y}e^{-xy} t\cos xt\,dx\\
&=\left[-\frac{1}{y}e^{-xy}\sin xt -\frac{t}{y^2}e^{-xy}\cos xt \right]_{0}^{\infty}-\frac{t^2}{y^2}\int_{0}^{\infty}e^{-xy} \sin xt\,dx\\
&=\left[\frac{-ye^{-xy}\sin xt-te^{-xy}\cos xt}{y^2} \right]_{0}^{\infty}-\frac{t^2}{y^2}\int_{0}^{\infty}e^{-xy} \sin xt\,dx\\
&=\frac{t}{y^2}-\frac{t^2}{y^2}\int_{0}^{\infty}e^{-xy} \sin xt\,dx
\end{align*}
thus
\begin{align*}
\int_{0}^{\infty}e^{-xy}\sin xt\,dx = \frac{t}{t^2+y^2}
\end{align*}
which then we apply it to (\ref{eq1}) to get
\begin{align*}
\lim_{\epsilon \to 0}F(\epsilon,t) &= \int_{0}^{\infty}\frac{t}{t^2+y^2}\,dy\\
&= \left[\tan^{-1}\frac{y}{t}\right]_{0}^{\infty}=\frac{\pi}{2}\text{sgn}(t)
\end{align*}


\end{enumerate}
\item


\item
\begin{enumerate}[(a)]
\item


\item



\item


\item
\end{enumerate}



\end{enumerate}


\end{document}